src/Turing.v
@@ -47,24 +47,23 @@ Require Import Coq.Logic.Classical_Prop.
     forall m i,
     (exists b, Exec m i b) \/ (forall b, ~ Exec m i b).
 
-  Inductive Prog :=
-  | Call: Prog -> input -> Prog
+  Inductive prog :=
     (**
      `Seq p1 f`: run p1, if p1 terminates, then
      run (f r) where `r` is a boolean that states if p1
      accepted or rejected its input.
     *)
-  | Seq: Prog -> (bool -> Prog) -> Prog
+  | Seq: prog -> (bool -> prog) -> prog
     (**
       Calls a machine with a given input
       (see Universal Turing Machines)
      *)
-  | Tur: machine -> Prog
+  | Call: machine -> input -> prog
     (**
       This Turing Machine just accepts/loops/rejects without
       any further operation.
       *)
-  | Ret: bool -> Prog
+  | Ret: bool -> prog
   .
 
   (**
@@ -72,134 +71,122 @@ Require Import Coq.Logic.Classical_Prop.
     We can run a program `p` and obtain a resul `r` with
     `Run p r`.
     *)
-  Inductive Run: Prog -> input -> bool -> Prop :=
-  | run_call:
-    forall p i j b,
-    Run p i b ->
-    Run (Call p i) j b 
+  Inductive Run: prog -> bool -> Prop :=
   | run_ret:
     (** We can directly return a result *)
-    forall b i,
-    Run (Ret b) i b
-  | run_tur:
+    forall b,
+    Run (Ret b) b
+  | run_call:
     (** Run a turing machine `m`. *)
     forall m i b,
     Exec m i b ->
-    Run (Tur m) i b
+    Run (Call m i) b
   | run_seq:
     (** If `p` terminates and returns `b`, then we can
        proceed with the execution of `q b`. *) 
-    forall p q b1 b2 i,
-    Run p i b1 ->
-    Run (q b1) i b2 ->
-    Run (Seq p q) i b2.
+    forall p q b1 b2,
+    Run p b1 ->
+    Run (q b1) b2 ->
+    Run (Seq p q) b2.
 
-  Inductive Halt : Prog -> input -> Prop :=
-  | halt_call:
-    forall p i j,
-    Halt p i ->
-    Halt (Call p i) j 
+  Inductive Halt : prog -> Prop :=
   | halt_ret:
     (** We can directly return a result *)
-    forall i b,
-    Halt (Ret b) i
-  | halt_tur:
+    forall b,
+    Halt (Ret b)
+  | halt_call:
     (** Run a turing machine `m`. *)
     forall m i b,
     Exec m i b ->
-    Halt (Tur m) i
+    Halt (Call m i)
   | halt_seq:
     (** If `p` terminates and returns `b`, then we can
        proceed with the execution of `q b`. *) 
-    forall p q b i,
-    Run p i b ->
-    Halt (q b) i ->
-    Halt (Seq p q) i.
+    forall p q b,
+    Run p b ->
+    Halt (q b) ->
+    Halt (Seq p q).
 
-  Inductive Loop: Prog -> input -> Prop :=
-  | loop_call:
-    forall p i j,
-    Loop p i ->
-    Loop (Call p i) j
+  Inductive Loop: prog -> Prop :=
   | loop_tur:
     (** Run a turing machine `m`. *)
     forall m i,
     (forall b, ~ Exec m i b) ->
-    Loop (Tur m) i
+    Loop (Call m i)
   | loop_seq_l:
     (** If `p` terminates and returns `b`, then we can
        proceed with the execution of `q b`. *) 
-    forall p q i,
-    Loop p i ->
-    Loop (Seq p q) i
+    forall p q,
+    Loop p ->
+    Loop (Seq p q)
   | loop_seq_r:
     (** If `p` terminates and returns `b`, then we can
        proceed with the execution of `q b`. *) 
-    forall p q b i,
-    Run p i b ->
-    Loop (q b) i ->
-    Loop (Seq p q) i.
+    forall p q b,
+    Run p b ->
+    Loop (q b) ->
+    Loop (Seq p q).
 
-  Inductive Negative p i : Prop :=
+  Inductive Negative (p:prog) : Prop :=
   | negative_run_false:
-    Run p i false ->
-    Negative p i
+    Run p false ->
+    Negative p
   | negative_loop:
-    Loop p i ->
-    Negative p i.
+    Loop p ->
+    Negative p.
 
   (** We define a notation for sequencing. *)
   Notation "'mlet' x <- e 'in' c" := (Seq e (fun x => c)) (at level 60, right associativity).
-  Definition ClosureOf (f:input -> input -> Prog) (c:input -> Prog) :=
-    forall param i b, Run (c param) i b <-> Run (f param i) i b.
+  Definition ClosureOf (f:input -> input -> prog) (c:input -> machine) :=
+    forall param i b, Run (f param i) b <-> Exec (c param) i b.
 
   Axiom closure_of :
-    forall p : input -> input -> Prog,
+    forall p : input -> input -> prog,
     exists R, ClosureOf p R.
-
-  Definition CodeOf f p :=
-    forall i b, Run p i b <-> Run (f i) i b.
-
-  Lemma code_of :
-    forall f : input -> Prog,
-    exists p, CodeOf f p.
-  Proof.
-    intros p. destruct (closure_of (fun _ => p)) as [R HR].
-    exists (R input_inhabited). unfold CodeOf. intros. eapply HR.
-  Qed.
 
   Lemma closure_of_run_rw {p} {f}:
     ClosureOf f p ->
-    forall j i b, Run (p j) i b <-> Run (f j i) i b.
+    forall j i b, Run (Call (p j) i) b <-> Run (f j i) b.
   Proof.
     unfold ClosureOf.
     intuition.
+    - apply H.
+      inversion_clear H0.
+      assumption.
+    - constructor.
+      apply H.
+      assumption.
   Qed.
+
+  Definition CodeOf (f:input -> prog) (m:machine) :=
+    forall (i:input) b, Run (f i) b <-> Exec m i b.
 
   Lemma code_of_run_rw {p} {f}:
     CodeOf f p ->
-    forall i b, Run p i b <-> Run (f i) i b.
+    forall i b, Run (Call p i) b <-> Run (f i) b.
   Proof.
     unfold CodeOf.
     intuition.
+    - inversion_clear H0.
+      apply H.
+      assumption.
+    - constructor.
+      apply H.
+      assumption.
   Qed.
 
-  Lemma run_call_rw:
-    forall p i j b,
-    Run (Call p j) i b <-> Run p j b.
+  Lemma code_of :
+    forall f : input -> prog,
+    exists m, CodeOf f m.
   Proof.
-    split; intros.
-    - inversion H; subst; auto.
-    - constructor; auto.
-  Qed.
-
-  Lemma halt_call_rw:
-    forall p i j,
-    Halt (Call p j) i <-> Halt p j.
-  Proof.
-    split; intros.
-    - inversion H; subst; auto.
-    - constructor; auto.
+    intros.
+    destruct (closure_of (fun x => f)) as (c, hc).
+    exists (c input_inhabited).
+    unfold CodeOf.
+    unfold ClosureOf in *.
+    intros.
+    rewrite hc.
+    reflexivity.
   Qed.
 
   (*----------------------------------------------------------------------------*)
@@ -207,19 +194,19 @@ Require Import Coq.Logic.Classical_Prop.
   Section RunLoopHalt.
 
     Lemma run_fun:
-      forall p i b1,
-      Run p i b1 ->
+      forall p b1,
+      Run p b1 ->
       forall b2,
-      Run p i b2 ->
+      Run p b2 ->
       b1 = b2.
     Proof.
-      intros p i r1 H; induction H; intros r' He;
+      intros p r1 H; induction H; intros r' He;
         inversion He; subst; clear He; auto;
         (* In each case we have a bunch of Run's that are solved
            by induction; we need to make sure we clear any dec's,
            so that we can advance to the next IH *) 
         repeat match goal with
-        | [ H1: Run ?q i ?b1, H2: Run ?q i ?b2 |- _] =>
+        | [ H1: Run ?q ?b1, H2: Run ?q ?b2 |- _] =>
           (
             assert (b1 = b2) by eauto ||
             assert (b2 = b1) by eauto
@@ -230,18 +217,12 @@ Require Import Coq.Logic.Classical_Prop.
     Qed.
 
     Lemma halt_to_run:
-      forall p i,
-      Halt p i ->
-      exists b, Run p i b.
+      forall p,
+      Halt p ->
+      exists b, Run p b.
     Proof.
       intros.
       induction H; try destruct IHHalt as (b, Hr).
-      (*- exists b.
-        constructor.
-        assumption.*)
-      - exists b.
-        constructor.
-        assumption.
       - exists b.
         constructor.
       - exists b.
@@ -253,24 +234,20 @@ Require Import Coq.Logic.Classical_Prop.
     Qed.
 
     Lemma run_to_halt:
-      forall p i b,
-      Run p i b ->
-      Halt p i.
+      forall p b,
+      Run p b ->
+      Halt p.
     Proof.
       intros.
       induction H.
-(*      - constructor.
-        assumption.*)
       - constructor.
-        assumption.
-      - constructor.
-      - eapply halt_tur; eauto.
+      - eapply halt_call; eauto.
       - eapply halt_seq; eauto.
     Qed.
 
     Lemma halt_rw:
-      forall p i,
-      Halt p i <-> exists b, Run p i b.
+      forall p,
+      Halt p <-> exists b, Run p b.
     Proof.
       split; intros.
       - auto using halt_to_run.
@@ -280,43 +257,26 @@ Require Import Coq.Logic.Classical_Prop.
 
     Lemma code_of_halt_rw {p} {f}:
       CodeOf f p ->
-      forall i, Halt p i <-> Halt (f i) i.
+      forall i, Halt (Call p i) <-> Halt (f i).
     Proof.
-      unfold CodeOf.
       intros.
       repeat rewrite halt_rw.
-      split; intros (x, Hx); exists x; apply H; auto.
+      split; intros (x, Hx); exists x.
+      - rewrite (code_of_run_rw H) in Hx.
+        assumption.
+      - rewrite (code_of_run_rw H).
+        assumption.
     Qed.
 
     Lemma halt_or_loop:
-      forall p i,
-      Halt p i \/ Loop p i.
+      forall p,
+      Halt p \/ Loop p.
     Proof.
       induction p; intros.
-        (*
-      - assert (H := H i i).
-        destruct H as [H| H].
-        + left.
-          constructor.
-          assumption.
-        + right.
-          constructor.
-          assumption.
-          *)
-      - assert (IHp := IHp i).
-        destruct IHp as [H|H]. {
-          left.
-          constructor.
-          assumption.
-        }
-        right.
-        constructor.
-        assumption.
-      - assert (IHp := IHp i).
-        destruct IHp as [IH|IH].
+      - destruct IHp as [IH|IH].
         + apply halt_to_run in IH.
           destruct IH as (b, IH).
-          assert (H := H b i).
+          assert (H := H b).
           destruct H as [H|H]. {
             left.
             econstructor; eauto.
@@ -338,9 +298,9 @@ Require Import Coq.Logic.Classical_Prop.
     Qed.
 
     Lemma loop_to_not_halt:
-      forall p i,
-      Loop p i ->
-      ~ Halt p i.
+      forall p,
+      Loop p ->
+      ~ Halt p.
     Proof.
       intros; induction H; intros N; inversion_clear N;
         try (contradict IHLoop; auto; fail).
@@ -354,17 +314,12 @@ Require Import Coq.Logic.Classical_Prop.
     Qed.
 
     Lemma halt_to_not_loop:
-      forall p i,
-      Halt p i ->
-      ~ Loop p i.
+      forall p,
+      Halt p ->
+      ~ Loop p.
     Proof.
       intros.
       induction H; intros N.
-     (* - inversion_clear N.
-        contradict H.
-        auto.*)
-      - inversion_clear N.
-        contradiction.
       - inversion_clear N.
       - inversion_clear N.
         contradict H.
@@ -380,20 +335,20 @@ Require Import Coq.Logic.Classical_Prop.
     Qed.
 
     Lemma not_halt_to_loop:
-      forall p i,
-      ~ Halt p i ->
-      Loop p i.
+      forall p,
+      ~ Halt p ->
+      Loop p.
     Proof.
       intros.
-      destruct (halt_or_loop p i). {
+      destruct (halt_or_loop p). {
         contradiction.
       }
       assumption.
     Qed.
 
     Lemma loop_rw:
-      forall p i,
-      Loop p i <-> ~ Halt p i.
+      forall p,
+      Loop p <-> ~ Halt p.
     Proof.
       split; intros. {
         auto using loop_to_not_halt.
@@ -403,7 +358,7 @@ Require Import Coq.Logic.Classical_Prop.
 
     Lemma code_of_loop_rw {p} {f}:
       CodeOf f p ->
-      forall i, Loop p i <-> Loop (f i) i.
+      forall i, Loop (Call p i) <-> Loop (f i).
     Proof.
       intros.
       repeat rewrite loop_rw.
@@ -411,30 +366,19 @@ Require Import Coq.Logic.Classical_Prop.
       reflexivity.
     Qed.
 
-    Lemma loop_call_rw:
-      forall p i j,
-      Loop (Call p j) i <-> Loop p j.
-    Proof.
-      split; intros. {
-        inversion_clear H.
-        assumption.
-      }
-      auto using loop_call.
-    Qed.
-
     Lemma run_exists:
-      forall p i,
-      (exists b, Run p i b) \/ Loop p i.
+      forall p,
+      (exists b, Run p b) \/ Loop p.
     Proof.
       intros.
-      destruct (halt_or_loop p i); auto.
+      destruct (halt_or_loop p); auto.
       rewrite halt_rw in *.
       auto.
     Qed.
 
     Lemma loop_alt_rw:
-      forall p i,
-      Loop p i <-> (forall b, ~ Run p i b).
+      forall p,
+      Loop p <-> (forall b, ~ Run p b).
     Proof.
       split; intros. {
         rewrite loop_rw in H.
@@ -451,8 +395,8 @@ Require Import Coq.Logic.Classical_Prop.
     Qed.
 
     Lemma negative_alt_rw:
-      forall p i,
-      Negative p i <-> (Run p i false \/ Loop p i).
+      forall p,
+      Negative p <-> (Run p false \/ Loop p).
     Proof.
       split; intros. { inversion_clear H; auto. }
       destruct H. { auto using negative_run_false. }
@@ -460,8 +404,8 @@ Require Import Coq.Logic.Classical_Prop.
     Qed.
 
     Lemma negative_rw:
-      forall p i,
-      Negative p i <-> ~ Run p i true.
+      forall p,
+      Negative p <-> ~ Run p true.
     Proof.
       split; intros. {
         intros N.
@@ -473,7 +417,7 @@ Require Import Coq.Logic.Classical_Prop.
         contradict H0.
         eapply run_to_halt; eauto.
       }
-      destruct (halt_or_loop p i). {
+      destruct (halt_or_loop p). {
         rewrite halt_rw in *.
         destruct H0 as ([], Ha); try contradiction.
         auto using negative_run_false.
@@ -483,7 +427,7 @@ Require Import Coq.Logic.Classical_Prop.
 
     Lemma code_of_negative_rw {p} {f}:
       CodeOf f p ->
-      forall i, Negative p i <-> Negative (f i) i.
+      forall i, Negative (Call p i) <-> Negative (f i).
     Proof.
       intros.
       repeat rewrite negative_rw.
@@ -493,14 +437,14 @@ Require Import Coq.Logic.Classical_Prop.
 
     Lemma closure_of_negative_rw {p} {f}:
       ClosureOf f p ->
-      forall i j, Negative (p j) i <-> Negative (f j i) i.
+      forall i j, Negative (Call (p j) i) <-> Negative (f j i).
     Proof.
       intros.
       repeat rewrite negative_rw.
       rewrite (closure_of_run_rw H).
       reflexivity.
     Qed.
-
+    (*
     Lemma negative_call_rw:
       forall p i j,
       Negative (Call p j) i <-> Negative p j.
@@ -523,21 +467,20 @@ Require Import Coq.Logic.Classical_Prop.
       rewrite loop_call_rw.
       assumption.
     Qed.
-
+*)
     Lemma run_true_or_negative:
-      forall p i,
-      Run p i true \/ Negative p i.
+      forall p,
+      Run p true \/ Negative p.
     Proof.
       intros.
-      destruct (run_exists p i) as [([], H)|H];
+      destruct (run_exists p) as [([], H)|H];
         auto;
         right;
         auto using negative_run_false, negative_loop.
     Qed.
 
     Lemma negative_ret:
-      forall i,
-      Negative (Ret false) i.
+      Negative (Ret false).
     Proof.
       intros.
       left.
@@ -546,94 +489,128 @@ Require Import Coq.Logic.Classical_Prop.
 
   End RunLoopHalt.
 
+  Parameter compile : prog -> machine.
+  Axiom compile_run_rw:
+    forall i p b,
+    Run (Call (compile p) i) b <-> Run p b.
+
   (** We also define a function to serialize a machine into a string (of type
       input). In the book, this corresponds to notation <M>. *)
-  Parameter encode_prog: Prog -> input.
+  Parameter encode_mach: machine -> input.
   (** Similarly, we have a function that takes a string and produces a machine.
       In the book, this corresponds to notation M = <M> *)
-  Parameter decode_prog: input -> Prog.
+  Parameter decode_mach: input -> machine.
   (** Decoding and encoding a machine yields the same machine. *)
-  Axiom decode_encode_prog_rw:
+  Axiom decode_encode_mach_rw:
     forall m,
-    decode_prog (encode_prog m) = m.
-  Axiom encode_decode_prog_rw:
-    forall w, encode_prog (decode_prog w) = w.
-  Axiom encode_prog_ext:
+    decode_mach (encode_mach m) = m.
+  Axiom encode_decode_mach_rw:
+    forall w, encode_mach (decode_mach w) = w.
+  Axiom encode_mach_ext:
     forall m1 m2,
-    encode_prog m1 = encode_prog m2 -> m1 = m2.
-
-  Axiom decode_prog_ext:
+    encode_mach m1 = encode_mach m2 -> m1 = m2.
+  Axiom decode_mach_ext:
     forall w1 w2,
-    decode_prog w1 = decode_prog w2 -> w1 = w2.
+    decode_mach w1 = decode_mach w2 -> w1 = w2.
 
   (** Given a machine and a string, encodes the pair as a string.
       In the book, this corresponds to notation <M, w>. *)
-  Definition encode_prog_input (M:Prog) (w:input) : input :=
-    encode_pair (encode_prog M, w).
+  Definition encode_mach_input (M:machine) (w:input) : input :=
+    encode_pair (encode_mach M, w).
 
   (** Given a string this function deserializes a pair M and w, given an encoded
       string <M,w>. *)
-  Definition decode_prog_input p := let (M, w) :=
-    decode_pair p in (decode_prog M, w).
+  Definition decode_mach_input p := let (M, w) :=
+    decode_pair p in (decode_mach M, w).
 
   (** Decoding and encoding a pair yields the same pair. *)
-  Lemma decode_encode_prog_input_rw:
+  Lemma decode_encode_mach_input_rw:
     forall M w,
-    decode_prog_input
-          (encode_prog_input M w) = (M, w).
+    decode_mach_input
+          (encode_mach_input M w) = (M, w).
   Proof.
     intros.
-    unfold decode_prog_input.
-    unfold encode_prog_input.
+    unfold decode_mach_input.
+    unfold encode_mach_input.
     rewrite decode_encode_pair_rw.
-    rewrite decode_encode_prog_rw.
+    rewrite decode_encode_mach_rw.
     reflexivity.
   Qed.
 
-  Lemma decode_prog_input_ext:
+  Lemma decode_mach_input_ext:
     forall i1 i2,
-    decode_prog_input i1 = decode_prog_input i2 ->
+    decode_mach_input i1 = decode_mach_input i2 ->
     i1 = i2.
   Proof.
-    unfold decode_prog_input.
+    unfold decode_mach_input.
     intros.
     destruct (decode_pair i1) as (M1, j1) eqn:R1.
     destruct (decode_pair i2) as (M2, j2) eqn:R2.
     inversion H; subst; clear H.
-    apply decode_prog_ext in H1.
+    apply decode_mach_ext in H1.
     subst.
     rewrite <- R1 in R2.
     apply decode_pair_ext in R2.
     auto.
   Qed.
 
-  Lemma decode_prog_input_rev:
+  Lemma decode_mach_input_rev:
     forall w M i,
-    decode_prog_input w = (M, i) ->
-    w = encode_prog_input M i.
+    decode_mach_input w = (M, i) ->
+    w = encode_mach_input M i.
   Proof.
     intros.
-    rewrite <- decode_encode_prog_input_rw in H.
-    apply decode_prog_input_ext in H.
+    rewrite <- decode_encode_mach_input_rw in H.
+    apply decode_mach_input_ext in H.
     assumption.
   Qed.
 
-  Lemma encode_prog_input_ext:
+  Lemma encode_mach_input_ext:
     forall M M' i i',
-    encode_prog_input M i = encode_prog_input M' i' -> M = M' /\ i = i'.
+    encode_mach_input M i = encode_mach_input M' i' -> M = M' /\ i = i'.
   Proof.
-    unfold encode_prog_input.
+    unfold encode_mach_input.
     intros.
     apply encode_pair_ext in H.
     inversion H; subst; clear H.
-    apply encode_prog_ext in H1.
+    apply encode_mach_ext in H1.
     auto.
   Qed.
 
   (** Let us define an abbreviation of the above functions. *)
   Notation "'<<' w1 ',' w2 '>>'" := (encode_pair w1 w2).
-  Notation "'[[' M ']]'" := (encode_prog M).
-  Notation "'<[' M , w ']>'" := (encode_prog_input M w).
+  Notation "'[[' M ']]'" := (encode_mach M).
+  Notation "'<[' M , w ']>'" := (encode_mach_input M w).
+
+
+  Section Examples.
+    Let a_tm_1 (s:input -> prog) : input -> prog :=
+    fun i =>
+      mlet b <- s <[ decode_mach i, i ]> in
+      if b then Ret false
+           else Ret true
+    .
+    Let a_tm_2 := fun p => 
+      let (M, w) := decode_mach_input p in
+      Call M w.
+
+    Let halt_tm (s:input -> prog) := fun p =>
+        let (M, w) := decode_mach_input p in
+        mlet b <- s p in
+        if b then Call M w else Ret false.
+
+    Let e_tm_1 p x := let (M, w) := decode_mach_input p in
+          if input_eq_dec x w then (
+            Call M w
+          ) else Ret false
+        .
+
+    Let e_tm_2 s (inner:input -> machine) := fun p =>
+        let (M, w) := decode_mach_input p in
+        mlet b <- s [[ inner p ]] in
+        if b then Ret false else Ret true.
+  End Examples.
+
 
   (** Define the equivalence of languages *)
   Definition Equiv (L1 L2:lang) :=
@@ -651,11 +628,11 @@ Require Import Coq.Logic.Classical_Prop.
       iff language L accepts i.
        *)
 
-  Definition Recognizes (p: input -> Prog) (L:lang) :=
-    forall i, Run (p i) i true <-> L i.
+  Definition Recognizes (p: input -> prog) (L:lang) :=
+    forall i, Run (p i) true <-> L i.
 
   Lemma recognizes_def {p} {L}:
-    (forall i, Run (p i) i true <-> L i) ->
+    (forall i, Run (p i) true <-> L i) ->
     Recognizes p L.
   Proof.
     intros.
@@ -665,7 +642,7 @@ Require Import Coq.Logic.Classical_Prop.
 
   Lemma recognizes_rw {p} {L}:
     Recognizes p L ->
-    forall i, Run (p i) i true <-> L i.
+    forall i, Run (p i) true <-> L i.
   Proof.
     unfold Recognizes.
     intuition.
@@ -673,8 +650,8 @@ Require Import Coq.Logic.Classical_Prop.
 
   Lemma recognizes_def_2:
     forall p (L:lang),
-    (forall i, Run (p i) i true -> L i) ->
-    (forall i, L i -> Run (p i) i true) ->
+    (forall i, Run (p i) true -> L i) ->
+    (forall i, L i -> Run (p i) true) ->
     Recognizes p L.
   Proof.
     intros.
@@ -782,7 +759,7 @@ Require Import Coq.Logic.Classical_Prop.
     Lemma recognizes_run_reject:
       forall p L i,
       Recognizes p L ->
-      Run (p i) i false ->
+      Run (p i) false ->
       ~ L i.
     Proof.
       intros.
@@ -792,23 +769,11 @@ Require Import Coq.Logic.Classical_Prop.
       inversion Hx.
     Qed.
 
-    Lemma c_recognizes_run_reject:
-      forall f p L i,
-      Recognizes f L ->
-      CodeOf f p ->
-      Run p i false ->
-      ~ L i.
-    Proof.
-      intros f p L i hr hc.
-      rewrite (code_of_run_rw hc).
-      eauto using recognizes_run_reject.
-    Qed.
-
     Lemma recognizes_run_accept:
       forall p L,
       Recognizes p L ->
       forall i,
-      Run (p i) i true ->
+      Run (p i) true ->
       L i.
     Proof.
       intros.
@@ -816,25 +781,12 @@ Require Import Coq.Logic.Classical_Prop.
       assumption.
     Qed.
 
-    Lemma c_recognizes_run_accept:
-      forall f p L i,
-      Recognizes f L ->
-      CodeOf f p ->
-      Run p i true ->
-      L i.
-    Proof.
-      intros f p L i hr hc.
-      rewrite (code_of_run_rw hc).
-      intros.
-      eapply recognizes_run_accept; eauto.
-    Qed.
-
     Lemma recognizes_not_accept:
       forall p L,
       Recognizes p L ->
       forall i,
       ~ L i ->
-      ~ Run (p i) i true.
+      ~ Run (p i) true.
     Proof.
       intros.
       intros N.
@@ -847,7 +799,7 @@ Require Import Coq.Logic.Classical_Prop.
       Recognizes p L ->
       forall i,
       ~ L i ->
-      Negative (p i) i.
+      Negative (p i).
     Proof.
       intros.
       rewrite negative_rw.
@@ -858,7 +810,7 @@ Require Import Coq.Logic.Classical_Prop.
       forall p L i,
       Recognizes p L ->
       L i ->
-      Run (p i) i true.
+      Run (p i) true.
     Proof.
       intros.
       apply H in H0.
@@ -869,7 +821,7 @@ Require Import Coq.Logic.Classical_Prop.
       forall p L,
       Recognizes p L ->
       forall i,
-      Loop (p i) i ->
+      Loop (p i) ->
       ~ L i.
     Proof.
       intros.
@@ -883,7 +835,7 @@ Require Import Coq.Logic.Classical_Prop.
       forall p L,
       Recognizes p L ->
       forall i,
-      Negative (p i) i ->
+      Negative (p i) ->
       ~ L i.
     Proof.
       intros.
@@ -892,11 +844,10 @@ Require Import Coq.Logic.Classical_Prop.
       - eauto using recognizes_run_loop.
     Qed.
 
-    Lemma recognizes_accept_rw:
-      forall p L,
+    Lemma recognizes_accept_rw {p} {L}:
       Recognizes p L ->
       forall i,
-      Run (p i) i true <-> L i.
+      Run (p i) true <-> L i.
     Proof.
       split; intros.
       - eapply recognizes_run_accept; eauto.
@@ -945,7 +896,7 @@ Require Import Coq.Logic.Classical_Prop.
     Lemma co_recognizes_run_accept:
       forall p L i,
       Recognizes p (compl L) ->
-      Run (p i) i true ->
+      Run (p i) true ->
       ~ L i.
     Proof.
       intros.
@@ -956,7 +907,7 @@ Require Import Coq.Logic.Classical_Prop.
       forall p L i,
       Recognizes p (compl L) ->
       L i ->
-      ~ Run (p i) i true.
+      ~ Run (p i) true.
     Proof.
       intros.
       intros N.
@@ -968,7 +919,7 @@ Require Import Coq.Logic.Classical_Prop.
       forall p L i,
       Recognizes p (compl L) ->
       ~ L i ->
-      Run (p i) i true.
+      Run (p i) true.
     Proof.
       intros.
       unfold compl in *.
@@ -984,11 +935,11 @@ Require Import Coq.Logic.Classical_Prop.
     (** We define a decider as any Turing Machine that returns either Accept or
         Reject, but not Loop. *)
 
-    Definition Decider (p:input -> Prog) := forall i, Halt (p i) i.
+    Definition Decider (p:input -> prog) := forall i, Halt (p i).
 
     Lemma decider_def:
       forall p,
-      (forall i, Halt (p i) i) ->
+      (forall i, Halt (p i)) ->
       Decider p.
     Proof.
       intros.
@@ -1053,7 +1004,7 @@ Require Import Coq.Logic.Classical_Prop.
     Lemma decides_run_reject:
       forall p L i,
       Decides p L ->
-      Run (p i) i false ->
+      Run (p i) false ->
       ~ L i.
     Proof.
       intros.
@@ -1064,7 +1015,7 @@ Require Import Coq.Logic.Classical_Prop.
     Lemma decides_run_accept:
       forall p L i,
       Decides p L ->
-      Run (p i) i true ->
+      Run (p i) true ->
       L i.
     Proof.
       intros.
@@ -1076,7 +1027,7 @@ Require Import Coq.Logic.Classical_Prop.
       forall p L i,
       Decides p L ->
       L i ->
-      Run (p i) i true.
+      Run (p i) true.
     Proof.
       intros.
       apply decides_to_recognizes in H.
@@ -1087,7 +1038,7 @@ Require Import Coq.Logic.Classical_Prop.
       forall p,
       Decider p ->
       forall i,
-      Halt (p i) i.
+      Halt (p i).
     Proof.
       intros.
       unfold Decider in *.
@@ -1097,7 +1048,7 @@ Require Import Coq.Logic.Classical_Prop.
     Lemma decider_to_run:
       forall p i,
       Decider p ->
-      exists b, Run (p i) i b.
+      exists b, Run (p i) b.
     Proof.
       intros.
       apply decider_to_halt with (i:=i) in H.
@@ -1108,7 +1059,7 @@ Require Import Coq.Logic.Classical_Prop.
     Lemma decides_to_run:
       forall p L i,
       Decides p L ->
-      exists b, Run (p i) i b.
+      exists b, Run (p i) b.
     Proof.
       intros.
       destruct H.
@@ -1121,7 +1072,7 @@ Require Import Coq.Logic.Classical_Prop.
       forall p L,
       Decides p L ->
       forall i,
-      Halt (p i) i.
+      Halt (p i).
     Proof.
       intros.
       destruct H.
@@ -1134,7 +1085,7 @@ Require Import Coq.Logic.Classical_Prop.
       Decides f L ->
       CodeOf f p ->
       forall i,
-      Halt p i.
+      Halt (Call p i).
     Proof.
       intros.
       rewrite (code_of_halt_rw H0).
@@ -1145,7 +1096,7 @@ Require Import Coq.Logic.Classical_Prop.
       forall p,
       Decider p ->
       forall i,
-      ~ Loop (p i) i.
+      ~ Loop (p i).
     Proof.
       intros.
       specialize (H i).
@@ -1155,8 +1106,8 @@ Require Import Coq.Logic.Classical_Prop.
     Lemma decider_not_reject:
       forall p i,
       Decider p ->
-      ~ Run (p i) i false ->
-      Run (p i) i true.
+      ~ Run (p i) false ->
+      Run (p i) true.
     Proof.
       intros.
       assert (H := H i).
@@ -1169,8 +1120,8 @@ Require Import Coq.Logic.Classical_Prop.
     Lemma decider_not_accept:
       forall p i,
       Decider p ->
-      ~ Run (p i) i true ->
-      Run (p i) i false.
+      ~ Run (p i) true ->
+      Run (p i) false.
     Proof.
       intros.
       assert (H := H i).
@@ -1194,11 +1145,11 @@ Require Import Coq.Logic.Classical_Prop.
       forall p L i,
       Decides p L ->
       ~ L i ->
-      Run (p i) i false.
+      Run (p i) false.
     Proof.
       intros.
       destruct H.
-      assert (Ha: Halt (p i) i) by auto using decider_to_halt.
+      assert (Ha: Halt (p i)) by auto using decider_to_halt.
       rewrite halt_rw in *.
       destruct Ha as (b, Ha).
       destruct b; auto.
@@ -1207,9 +1158,9 @@ Require Import Coq.Logic.Classical_Prop.
     Qed.
 
     Lemma run_seq_rw:
-      forall p q i b,
-      Run (Seq p q) i b <-> (
-        (exists b', Run p i b' /\ Run (q b') i b)
+      forall p q b,
+      Run (Seq p q) b <-> (
+        (exists b', Run p b' /\ Run (q b') b)
       ).
     Proof.
       split; intros. {
@@ -1221,9 +1172,9 @@ Require Import Coq.Logic.Classical_Prop.
     Qed.
 
     Lemma run_seq_pre_rw:
-      forall p q i b b',
-      Run p i b' ->
-      Run (Seq p q) i b <-> Run (q b') i b.
+      forall p q b b',
+      Run p b' ->
+      Run (Seq p q) b <-> Run (q b') b.
     Proof.
       intros.
       rewrite run_seq_rw.
@@ -1241,7 +1192,7 @@ Require Import Coq.Logic.Classical_Prop.
       forall f P,
       Decides f P ->
       forall i,
-      Run (f i) i false <-> ~ P i.
+      Run (f i) false <-> ~ P i.
     Proof.
       split; intros. {
         eauto using decides_run_reject.
@@ -1253,7 +1204,7 @@ Require Import Coq.Logic.Classical_Prop.
       forall f P,
       Decides f P ->
       forall i,
-      Run (f i) i true <-> P i.
+      Run (f i) true <-> P i.
     Proof.
       split; intros. {
         eapply decides_run_accept; eauto.
@@ -1262,10 +1213,10 @@ Require Import Coq.Logic.Classical_Prop.
     Qed.
 
     Lemma halt_seq_alt:
-      forall p i (c:bool -> Prog),
-      Halt p i ->
-      (forall (b:bool), Run p i b -> Halt (c b) i) -> 
-      Halt (Seq p c) i.
+      forall p (c:bool -> prog),
+      Halt p ->
+      (forall (b:bool), Run p b -> Halt (c b)) -> 
+      Halt (Seq p c).
     Proof.
       intros.
       rewrite halt_rw in H.
@@ -1274,26 +1225,25 @@ Require Import Coq.Logic.Classical_Prop.
     Qed.
 
     Lemma halt_seq_decider:
-      forall p i j (c:bool -> Prog),
+      forall p j (c:bool -> prog),
       Decider p ->
-      (forall (b:bool), Run (p j) j b -> Halt (c b) i) -> 
-      Halt (Seq (Call (p j) j) c) i.
+      (forall (b:bool), Run (p j) b -> Halt (c b)) -> 
+      Halt (Seq (p j) c).
     Proof.
       intros.
       apply halt_seq_alt. {
-        constructor.
-        eauto.
+        apply H.
       }
       intros.
-      inversion_clear H1.
-      eauto.
+      apply H0.
+      assumption.
     Qed.
 
     Lemma halt_seq_decides:
-      forall p i j L (c:bool -> Prog),
+      forall p j L (c:bool -> prog),
       Decides p L ->
-      (forall (b:bool), Run (p j) j b -> Halt (c b) i) -> 
-      Halt (Seq (Call (p j) j) c) i.
+      (forall (b:bool), Run (p j) b -> Halt (c b)) -> 
+      Halt (Seq (p j) c).
     Proof.
       intros.
       apply halt_seq_decider; auto.
@@ -1309,18 +1259,9 @@ Require Import Coq.Logic.Classical_Prop.
   match goal with
   | [ H: _ |- _ ] =>
     match type of H with
-      | Run (Call _ _) _ _ => idtac
-(*       | Run (Read _) _ _ => idtac *)
-      | Run (Tur _) _ _ => idtac 
-      | Run (Ret _) _ _ => idtac
-      | Loop (Call _ _) _ => idtac
-(*       | Loop (Read _) _ => idtac *)
-      | Loop (Tur _) _ => idtac
-      | Loop (Ret _) _ => idtac
-      | Halt (Call _ _) _ => idtac
-(*       | Halt (Read _) _ => idtac *)
-      | Halt (Tur _) _ => idtac
-      | Halt (Ret _) _ => idtac
+      | Run (Ret _) _ => idtac
+      | Loop (Ret _) => idtac
+      | Halt (Ret _) => idtac
       | _ => fail
     end;
     inversion H; subst; clear H
@@ -1342,27 +1283,28 @@ Require Import Coq.Logic.Classical_Prop.
     end.
 
   Ltac run_simpl_rw := (
-      rewrite decode_encode_prog_input_rw in * ||
+      rewrite decode_encode_mach_input_rw in * ||
       rewrite decode_encode_pair_rw in * ||
       rewrite encode_decode_pair_rw in * ||
-      rewrite decode_encode_prog_rw in * ||
-      rewrite encode_decode_prog_rw in *).
+      rewrite decode_encode_mach_rw in * ||
+      rewrite encode_decode_mach_rw in * ||
+      rewrite compile_run_rw in *).
 
 
   Ltac run_simpl_norm :=
     match goal with
     | [ H: ?x = ?x |- _] => clear H
-    | [ H1: Negative ?p ?i, H2: Run ?p ?i true |- _ ] =>
+    | [ H1: Negative ?p, H2: Run ?p true |- _ ] =>
       rewrite negative_rw in H1; contradiction
-    | [ H1: Run ?p ?i _, H2: Loop ?p ?i |- _ ] =>
+    | [ H1: Run ?p _, H2: Loop ?p |- _ ] =>
       apply run_to_halt in H1;
       rewrite loop_rw in H2; contradiction 
-    | [ H1: Halt ?p ?i, H2: Loop ?p ?i |- _ ] =>
+    | [ H1: Halt ?p , H2: Loop ?p  |- _ ] =>
       rewrite loop_rw in H2; contradiction
-    | [ H1: Run ?m ?i ?r1, H2: Run ?m ?i ?r2  |- _] =>
+    | [ H1: Run ?m ?r1, H2: Run ?m ?r2  |- _] =>
       assert (r1 = r2) by eauto using run_fun;
       subst; clear H1
-    | [ H1: Exec ?m ?i ?r1, H2: Exec ?m ?i ?r2  |- _] =>
+    | [ H1: Exec ?m ?r1, H2: Exec ?m ?r2  |- _] =>
       assert (r1 = r2) by eauto using exec_fun;
       subst; clear H1
     | [ H: true = _ |- _ ] => symmetry in H
